\documentclass{beamer}

\usepackage{amsmath,cancel}
\usepackage{graphicx}
\usepackage{color}
\usepackage{alltt}

\newcommand{\sect}[1]{
\section{#1}
\begin{frame}[fragile]\frametitle{#1}
}
 
\begin{document}

\sect{Divide and Conquer Matrix Multiply}

\begin{align*}
  T(1) &= c\\
  T(n) &= 8T(n/2) + cn^2
  \\\\
  T(n) &= \cancel{8T(n/2)} + c(n)^2\\
  \cancel{8T(n/2)} &= \cancel{8^2T(n/2^2)} + 8c(n/2)^2 \\
  \cancel{8^2T(n/2^2)} &= \cancel{8^3T(n/2^3)} + 8^2c(n/2^2)^2\\
  \cancel{8^3T(n/2^3)} &= \cancel{8^4T(n/2^4)} + 8^3c(n/2^3)^2\\
  &\ldots\\
  \cancel{8^{\lg n - 1}T(n/2^{\lg n - 1})} &= 8^{\lg n}T(1) + 8^{\lg n - 1}c(n/2^{\lg n - 1})^2
\end{align*}

\end{frame}
\sect{Divide and Conquer Matrix Multiply}
\begin{align*}
  T(n) &=  c8^{\lg n} + \sum_{i=0}^{\lg n -1}8^ic(n/2^{i})^2\\
  &=   cn^{\lg 8} + cn^2\sum_{i=0}^{\lg n -1}\frac{8^i}{4^i}\\
  &=   cn^3 + cn^2\sum_{i=0}^{\lg n -1}2^i\\
  &=   cn^3 + cn^2\frac{2^{\lg n} - 1}{2-1}\\
  &=   cn^3 + cn^2(n^{\lg 2} - 1)\\
  &=   cn^3 + cn^2(n - 1)\\
  &= \Theta(n^3)
  \end{align*}
\end{frame}

\sect{Strassen Matrix Multiply}
\begin{align*}
  T(1) &= c\\
  T(n) &= 7T(n/2) + cn^2
\end{align*}

\begin{align*}
  T(n) &= \cancel{7T(n/2)} + c(n)^2\\
  \cancel{7T(n/2)} &= \cancel{7^2T(n/2^2)} + 7c(n/2)^2 \\
  \cancel{7^2T(n/2^2)} &= \cancel{7^3T(n/2^3)} + 7^2c(n/2^2)^2\\
  \cancel{7^3T(n/2^3)} &= \cancel{7^4T(n/2^4)} + 7^3c(n/2^3)^2\\
  &\ldots\\
  \cancel{7^{\lg n - 1}T(n/2^{\lg n - 1})} &= 7^{\lg n}T(1) + 7^{\lg n - 1}c(n/2^{\lg n - 1})^2
  \end{align*}
\begin{align*}
  T(n) &=  c7^{\lg n} + \sum_{i=0}^{\lg n -1}7^ic(n/2^{i})^2\\
\end{align*}
\end{frame}

\sect{Solve the summation}
\begin{align*}
  T(n) &=  c7^{\lg n} + \sum_{i=0}^{\lg n -1}7^ic(n/2^{i})^2\\
  &=   cn^{\lg 7} + cn^2\sum_{i=0}^{\lg n -1}\frac{7^i}{4^i}\\
  &=   cn^{\lg 7} + cn^2\sum_{i=0}^{\lg n -1}(7/4)^i\\
\end{align*}
\end{frame}

\sect{Solve the summation}
\begin{align*}
    cn^{\lg 7} + cn^2\sum_{i=0}^{\lg n -1}(7/4)^i
  &=   cn^{\lg 7} + cn^2\left(\frac{(7/4)^{\lg n} - 1}{(7/4)-1}\right)\\
  &=   cn^{\lg 7} + cn^2\left(\frac{n^{\lg 7/4} - 1}{3/4}\right)\\
  &=   cn^{\lg 7} + \frac{4cn^2}{3}\left(n^{\lg 7/4} - 1\right)\\
  &=   cn^{\lg 7} + \frac{4cn^2}{3}\left(n^{\lg 7-\lg 4} - 1\right)\\
  &=   cn^{\lg 7} + \frac{4cn^2}{3}\left(\frac{n^{\lg 7}}{n^{\lg 4}} - 1\right)\\
  &=   cn^{\lg 7} + \frac{4c}{3}\left(n^{\lg 7} - n^2\right)\\
  &= O(n^{\lg 7})\\
  &= o(n^{2.81}) = o(n^3)
  \end{align*}

\end{frame}
\end{document}





