\documentclass{article}
\pagestyle{empty}
\usepackage{fullpage}
\usepackage{polynom}

\usepackage{amsmath}
\usepackage{graphicx}
\usepackage{color}
\usepackage{alltt}
\newcommand{\red}[1]{{\color{red}#1}}
\newcommand{\cyan}[1]{{\color{cyan}#1}}
\newcommand{\blue}[1]{{\color{blue}#1}}
\newcommand{\magenta}[1]{{\color{magenta}#1}}
\newcommand{\yellow}[1]{{\color{yellow}#1}}
\newcommand{\green}[1]{{\color{green}#1}}
 
\newcommand{\bkt}[1]{\langle \mbox{ #1 } \rangle}
\newcommand{\br}{\mbox{~}|\mbox{~}}
 
\newcommand{\ns}[1]{\newpage\noindent {\bf #1}}
 
\begin{document}
 
\huge

{\bf Summation Facts}
\begin{eqnarray*}
\sum_{i=m}^n c &=& (n - m + 1)c 
\\\\
\sum_{i=m}^n ca_i &=& c\sum_{i=m}^n a_i 
\\\\
\sum_{i=m}^n (a_i + b_i) &=& \sum_{i=m}^n a_i + \sum_{i=m}^n + b_i
\\\\
\sum_{i=m}^n a_{i+k} &=& \sum_{i=m+k}^{n+k} a_{i}
\\\\
\sum_{i=m}^n a_{i}x^{i+k} &=& x^k \sum_{i=m}^{n} a_{i}x^i
\\\\
\sum_{i=m}^n (a_i - a_{i-1}) &=& a_n - a_{m-1}
\end{eqnarray*}

\ns{Sum of 1}

Use telescoping:
\begin{eqnarray*}
\sum_{i=m}^n (a_i - a_{i-1}) &=& a_n - a_{m-1}
\end{eqnarray*}
Let $a_i = i$:
\begin{eqnarray*}
  \sum_{i=1}^n (a_i - a_{i-1}) &=&  \sum_{i=1}^n (i - (i - 1))
  \\
  &=&  \sum_{i=1}^n 1
  \\
   &=&  a_n - a_{m-1}
  \\
  &=& n - 0
  \\
  &=& n
\end{eqnarray*}

\ns{Sum of $i$}
\[
\begin{array}{cccccccccc}
 & \sum_{i=1}^n i &=& 1 &+& 2 &+& \ldots  &+& n
\\
+&  \sum_{i=1}^n i  &=& n &+& n-1 &+& \ldots  &+& 1
\\
\multicolumn{10}{c}{\hrulefill}
\\
 &&=& n+1 &+& n+1 &+& \ldots  &+& n+1
  \\
 & &=& \multicolumn{3}{l}{n(n+1)}
  \\\\\\
\Rightarrow&  \sum_{i=1}^n i &=& \multicolumn{3}{l}{{n(n+1)}/{2}}
\end{array}
\]

\ns{Sum of $i$}
\begin{eqnarray*}
  n^2 &=& n^2 - 0^2
  \\
  &=& \sum_{i=1}^n (i^2 - (i-1)^2)
  \\
  &=& \sum_{i=1}^n (2i - 1)
  \\
  &=& 2\sum_{i=1}^n i - \sum_{i=1}^n 1
  \\
  &=& 2\sum_{i=1}^n i - n
  \\
  n^2 + n   &=& 2\sum_{i=1}^n i
  \\
  \sum_{i=1}^{n} i &=& \frac{n^2+n}{2}
  \\
   &=& \frac{n(n+1)}{2}
\end{eqnarray*}

\ns{Sum of $i$}
\begin{eqnarray*}
\sum_{i=1}^{n+1}i^2 &=& \sum_{i=1}^{n}i^2 + (n+1)^2 \\
                 &=& \sum_{i=1}^{n}i^2 + n^2 + 2n + 1 \\
\sum_{i=1}^{n+1}i^2 &=& \sum_{i=0}^{n}(i+1)^2 \\
                 &=& \sum_{i=0}^{n}(i^2 + 2i + 1) \\
                 &=& \sum_{i=0}^{n}i^2 + \sum_{i=0}^{n}2i + \sum_{i=0}^{n}1 \\
                 &=& \sum_{i=0}^{n}i^2 + \sum_{i=0}^{n}2i + n+1 \\
\sum_{i=1}^{n}i^2 + n^2 + 2n + 1 
    &=& \sum_{i=0}^{n}i^2 + \sum_{i=0}^{n}2i + n+1 \\
 n^2 + 2n + 1  &=&  \sum_{i=0}^{n}2i + n+1 \\
 \sum_{i=0}^{n}2i &=& n^2 + n \\
 \sum_{i=0}^{n}i &=& n(n+1)/2
\end{eqnarray*}

\ns{Sum of Odd Numbers}
\begin{eqnarray*}
1 + 3 + \ldots + (2n+1) &=& \sum_{i=0}^n (2i+1) 
\\
&=& \sum_{i=0}^n 2i + \sum_{i=0}^n 1
\\
&=& 2\sum_{i=0}^n i + (n+1)
\\
&=& 2n(n+1)/2 + (n+1)
\\
&=& (n+1)^2
\end{eqnarray*}

\ns{Geometric Sum}
\begin{eqnarray*}
  S_n &=& 1 + a + a^2 + \ldots + a^n
  \\
  &=& \sum_{i=0}^n a^i
  \\
  S_{n+1} &=& (1 + a + a^2 + \ldots + a^n) + a^{n+1}
  \\
  &=& S_{n} + a^{n+1}
  \\
  S_{n+1} &=& 1 + (a + a^2 + \ldots + a^n + a^{n+1})
  \\
  &=& 1 + a(1 + a + a^2  +  \ldots + a^n)
  \\
  &=& 1 + aS_n
  \\
  &\Rightarrow&
  \\
  S_n + a^{n+1} &=& 1 + aS_n
  \\
  &\Rightarrow&
  \\
  \sum_{i=0}^n a^i &=& S_n
  \\
  &=& \frac{a^{n+1} - 1}{a-1}
\end{eqnarray*}


\ns{Geometric Sum}
\begin{eqnarray*}
  (a-1)\sum_{i=0}^n a^i &=& \sum_{i=0}^n (a^{i+1} - a^i)
  \\
  &=&  \sum_{j=1}^{n+1} (a^j - a^{j-1})
  \\
  &=& a^{n+1} - a^0
  \\
  &=& a^{n+1} - 1
\end{eqnarray*}

Also do division:

\[
\polyset{vars=a}
\polylongdiv{a^5-1}{a-1}
\]

\ns{Sum of $ia^i$}
\begin{eqnarray*}
  S_n = \sum_{i=1}^n ia^i 
    &=& 1+a+2a^2+\ldots + na^n
  \\
  S_{n+1} = \sum_{i=1}^{n+1} ia^i
  &=&  \sum_{i=1}^n ia^i + (n+1)a^{n+1}
  \\
  &=& S_n + (n+1)a^{n+1}
  \\
  S_{n+1} = \sum_{i=1}^{n+1} ia^i
  &=& \sum_{i=0}^{n} (i+1)a^{i+1}
  \\
  &=& \sum_{i=0}^{n} ia^{i+1} + \sum_{i=0}^{n} a^{i+1}
  \\
  &=& a\sum_{i=0}^{n} ia^{i} + a\sum_{i=0}^{n} a^{i}
  \\
  &=& aS_n + a(a^{n+1} - 1)/(a-1)
  \\
  &\Rightarrow&
  \\
  S_n + (n+1)a^{n+1}  &=& aS_n + a(a^{n+1} - 1)/(a-1)
  \\
  &\Rightarrow&
  \\
  S_n  &=& \frac{a - (n+1)a^{n+1} + na^{n+2}}{(a-1)^2}
\end{eqnarray*}
  
\ns{Sum of $ia^{i-1}$}

Don't forget your calculus!
\begin{eqnarray*}
  \frac{d}{dx}(f+g) &=& \frac{df}{dx} + \frac{dg}{dx}
  \\\\\\
  \sum_{i=0}^n ia^{i-1} &=&   \sum_{i=0}^n \frac{d}{da} (a^i)
  \\
  &=&   \frac{d}{da}  \sum_{i=0}^n (a^i)
  \\
  &=&   \frac{d}{da} \left(  \frac{a^{n+1} - 1}{a-1} \right)
\end{eqnarray*}

\ns{Sum of $i^2$}
\begin{eqnarray*}
  \sum_{i=1}^{n+1} i^3 &=& \sum_{i=1}^n i^3 + (n+1)^3
  \\
  \sum_{i=1}^{n+1} i^3 &=&\sum_{i=0}^{n} (i+1)^3
  \\
  &=&  \sum_{i=0}^{n} (i^3 + 3i^2 + 3i +1)
  \\
  &=& \sum_{i=0}^{n} i^3 +
      \sum_{i=0}^{n} 3i^2 + 
      \sum_{i=0}^{n} 3i + 
      \sum_{i=0}^{n} 1
  \\
  &=& \sum_{i=1}^{n} i^3 +
      3\sum_{i=1}^{n} i^2 + 
      3\sum_{i=1}^{n} i + 
      (n+1)      
  \\
  &=& \sum_{i=1}^{n} i^3 +
      3\sum_{i=1}^{n} i^2 + 
      3\frac{n(n+1)}{2} +
      (n+1)
  \\\\\\
  &\Rightarrow&
  \\
  (n+1)^3 &=&       3\sum_{i=1}^{n} i^2 + 
      3\frac{n(n+1)}{2} +
      (n+1)
  \\\\\\
  &\Rightarrow&
  \\
  \sum_{i=1}^n i^2 &=& \frac{n(n+1)(2n+1)}{6}
\end{eqnarray*}

\ns{Harmonic series}

\begin{align*}
\sum_{n=1}^{\infty}\frac1n &= 1 + \frac{1}{2} + \frac13 + \frac14 + \frac15 + \cdots
\\
\sum_{n=1}^{2^k} \frac1n &\geq 1 + \frac{k}{2} & k > 0
\\
\sum_{n=1}^{k} \frac1n &< \ln(k) + 1
\end{align*}

\ns{Change of variables}
\begin{align*}
\sum_{i=1}^{n} \frac{1}{n-i+1}
&=
\sum_{i=1}^{i=n} \frac{1}{n-i+1} &\mbox{let $i=n-j$}\\
&=
\sum_{n-j=1}^{n-j=n} \frac{1}{n-(n-j)+1}\\
&=
\sum_{j=n-1}^{j=0} \frac{1}{j+1}\\
&=
\sum_{j=0}^{n-1} \frac{1}{j+1}\\
&=
\sum_{j=1}^{n} \frac{1}{j}\\
&=
\sum_{i=1}^{n} \frac{1}{i}
\end{align*}
Which is the Harmonic series.


\ns{Consider using Sympy}

{\LARGE
\begin{verbatim}
>>> from sympy import summation, oo, symbols, latex, log

>>> i,n,m = symbols('i n m', integer=True)

>>> summation(2*i + 1, (i, 0, n-1))
n**2

>>> summation(1/2**i, (i,0,oo))
2

>>> summation(i, (i, 0, n), (n, 0, m))
m**3/6 + m**2/2 + m/3

>>> print(latex(summation(i, (i,0,n), (n,0,m))))
\frac{m^{3}}{6} + \frac{m^{2}}{2} + \frac{m}{3}

>>> print(latex(summation(1/log(n)**n, (n, 2, oo))))
\sum_{n=2}^{\infty} \log^{- n}{\left (n \right )}
\end{verbatim}
}

\end{document}







